erasure/theories/ErasureCorrectness.v
@@ -472,8 +472,39 @@ Proof.
     + exists tBox. split. 2:econstructor; eauto.
       econstructor. eapply Is_type_eval; eauto.
     + auto.
-  - inv isdecl.
-  - inv isdecl.
+  - destruct i; discriminate.
+  - destruct i; discriminate.
+  - destruct Σ as (Σ, univs).
+    unfold erases_global in Heg.
+    assert (Σ ;;; [] |- tConst c u ▷ res) by eauto.
+    eapply inversion_Const in Hty as (? & ? & ? & ? & ?).
+    inv He.
+    + assert (H' := H).
+      eapply lookup_env_erases in H; eauto.
+      destruct H as (decl' & ? & ?).
+      unfold erases_constant_body in H2. rewrite H0 in *.
+      destruct ?; try tauto. cbn in *.
+      eapply declared_constant_inj in d; eauto; subst.
+      edestruct IHeval.
+      * cbn in *.
+        eapply PCUICWeakeningEnv.declared_constant_inv in H'; eauto.
+        unfold on_constant_decl in H'. rewrite H0 in H'. red in H'.
+        eapply typing_subst_instance in H'; eauto.
+        eapply PCUICWeakeningEnv.weaken_env_prop_typing.
+      * eapply PCUICWeakeningEnv.declared_constant_inv in H'; eauto.
+        unfold on_constant_decl in H'. rewrite H0 in H'. cbn in *.
+        2:eapply PCUICWeakeningEnv.weaken_env_prop_typing.
+        eapply erases_subst_instance_constr in H'; eauto.
+      * destruct H3. exists x0. split; eauto. econstructor; eauto.
+    + exists tBox. split. econstructor.
+      eapply Is_type_eval. 3: eassumption. eauto. eauto. econstructor. eauto.
+    + auto.
+
+  - destruct Σ as (Σ, univs).
+    unfold erases_global in Heg.
+    (* Axiom free hyp is missing *)
+    admit.
+
   - assert (Hty' := Hty).
     assert (Σ ;;; [] |- tCase (ind, pars) p discr brs ▷ res) by eauto.
     eapply inversion_Case in Hty' as (u' & args' & mdecl & idecl & pty & indctx & pctx & ps & btys & ? & ? & ? & ? & ? & ? & ? & ? & ?).
@@ -617,29 +648,91 @@ Proof.
     + admit.
     + auto.
     + auto.
+  - pose (Hty' := Hty).
+    eapply inversion_Proj in Hty' as (? & ? & ? & [] & ? & ? & ? & ? & ?).
+    inv He.
+    + eapply IHeval1 in H6 as (vc' & Hvc' & Hty_vc'); eauto.
+      eapply erases_mkApps_inv in Hvc'; eauto.
+      2: eapply subject_reduction_eval; eauto.
+      destruct Hvc' as [ (? & ? & ? & ? & [] & ? & ? & ?) | (? & ? & ? & ? & ?)]; subst.
+      * exists tBox. split.
+
+        eapply Is_type_app in X as []; eauto. 2:{ rewrite mkApps_nested. eapply subject_reduction_eval; eauto. }
+        rewrite mkApps_nested in X.
+
+        eapply tConstruct_no_Type in X. eapply H4 in X as [? []]; eauto.
+        2: now destruct d. 2: now exists []; destruct Σ.
+
+        econstructor.
+        eapply Is_type_eval. eauto. eauto.
+        eapply nth_error_all.
+        erewrite nth_error_skipn. reflexivity. eassumption.
+        eapply All_impl. assert (pars = ind_npars x0). destruct d as (? & ? & ?). now rewrite H8. subst.
+        eassumption.
+        eapply isErasable_Proof. eauto.
+
+        eapply eval_proj_box.
+        pose proof (Ee.eval_to_value _ _ _ Hty_vc').
+        eapply value_app_inv in H2. subst. eassumption.
+      * rename H4 into Hinf.
+        eapply Forall2_nth_error_Some in H5 as (? & ? & ?); eauto.
+        assert (Σ ;;; [] |- mkApps (tConstruct i k u) args : mkApps (tInd i x) x2).
+        eapply subject_reduction_eval; eauto.
+        eapply type_mkApps_inv in X as (? & ? & [] & ?); eauto.
+        eapply typing_spine_inv in t2 as []; eauto.
+        eapply IHeval2 in H4 as (? & ? & ?); eauto.
+        inv H3.
+        -- exists x9. split; eauto. econstructor. eauto.
+           rewrite <- nth_default_eq. unfold nth_default. now rewrite H2.
+        -- exists tBox. split.
+
+
+           eapply Is_type_app in X as []; eauto. 2:{ eapply subject_reduction_eval. 3: eauto. eauto. eauto. }
+
+           eapply tConstruct_no_Type in X. eapply Hinf in X as [? []]; eauto.
+           2: now destruct d. 2: now exists []; destruct Σ.
+
+           econstructor.
+           eapply Is_type_eval. eauto. eauto.
+           eapply nth_error_all.
+           erewrite nth_error_skipn. reflexivity. eassumption.
+           eapply All_impl. assert (pars = ind_npars x0). destruct d as (? & ? & ?). now rewrite H8. subst.
+           eassumption.
+           eapply isErasable_Proof. eauto.
+
+           eapply eval_proj_box.
+           pose proof (Ee.eval_to_value _ _ _ Hty_vc').
+           eapply value_app_inv in H3. subst. eassumption.
+    + exists tBox. split. econstructor.
+      eapply Is_type_eval. 3: eassumption. eauto. eauto. econstructor. eauto.
+    + auto.
+
   - assert (Hty' := Hty).
-    assert (Hunf := H).
+    assert (Hunf := H0).
     assert (Hcon := H1).
-    assert (Σ ;;; [] |- mkApps (tFix mfix idx) args ▷ res) by eauto.
+    assert (Σ ;;; [] |- mkApps f args ▷ res) by eauto.
     eapply type_mkApps_inv in Hty' as (? & ? & [] & ?); eauto.
     assert (HT := t).
+    eapply subject_reduction_eval in t; eauto.
     eapply inversion_Fix in t as (? & ? & ? & ? & ? & ?).
-    unfold unfold_fix in H. rewrite e in H. inv H.
+    unfold unfold_fix in H0. rewrite e in H0.
+    destruct ?. 2:{ discriminate. } all:eauto. inv H0.
 
     eapply erases_mkApps_inv in He as [(? & ? & ? & ? & [] & ? & ? & ?) | (? & ? & ? & ? & ?)]; eauto.
-    + subst. assert (X100 := X1). eapply Is_type_app in X100 as[].
+    + subst. assert (X100 := Hty).
+      rewrite <- mkApps_nested in X100. eapply Is_type_app in X100 as[]. all:eauto.
       exists tBox. split. 2:{
         assert (exists x5, Forall2 (EWcbvEval.eval Σ') x4 x5) as [x5]. {
-          eapply All2_app_inv in H0 as ([] & ? & ?). destruct p.
+          eapply All2_app_inv in H3 as ([] & ? & ?). destruct p.
           clear a0. subst.
           assert (forall x n, nth_error x3 n = Some x -> ∑ T,  Σ;;; [] |- x : T).
           { intros. eapply typing_spine_inv with (arg := n + #|x2|) in t0 as [].
             2:{ rewrite nth_error_app2. 2:omega. rewrite Nat.add_sub. eassumption. }
             eauto.
           } 
-          clear - X3 a1 H5. revert X3 x4 H5; induction a1; intros.
-          ** inv H5. exists []; eauto.
-          ** inv H5. destruct (X3 x 0 eq_refl).
+          clear - X3 a1 H6. revert X3 x4 H6; induction a1; intros.
+          ** inv H6. exists []; eauto.
+          ** inv H6. destruct (X3 x 0 eq_refl).
              eapply r in t as (? & ? & ?); eauto.
              eapply IHa1 in H3 as (? & ?); eauto.
              intros. eapply (X3 x2 (S n)). eassumption.
@@ -647,13 +740,16 @@ Proof.
         eapply eval_box_apps. eassumption. econstructor; eauto. }
       econstructor.
       eapply Is_type_eval. eauto. eassumption.
-      rewrite <- mkApps_nested.  eassumption. eauto. econstructor.
-      rewrite mkApps_nested; eauto.
+      rewrite <- mkApps_nested.  eassumption.
     + subst.
-      destruct ?; inv H4.
-      inv H3.
-      * assert (Hmfix' := H7).
-        eapply All2_nth_error_Some in H7 as (? & ? & ? & ? & ?); eauto.
+      specialize (IHeval1 _ HT _ H5).
+      destruct IHeval1 as [v' [fixv' x2v']].
+      admit.
+      (*
+
+      inv fixv'.
+      * assert (Hmfix' := H4).
+        eapply All2_nth_error_Some in H4 as (? & ? & ? & ? & ?); eauto.
         destruct x1. cbn in *. subst.
 
         enough(Σ;;; [] ,,, subst_context (fix_subst mfix) 0 [] |- PCUICLiftSubst.subst (fix_subst mfix) 0 dbody ⇝ℇ subst (ETyping.fix_subst mfix') 0 (Extract.E.dbody x2)). clear e3. rename H into e3.
@@ -751,93 +847,46 @@ Proof.
         } 
         
         eapply eval_box_apps. eauto. econstructor. eauto. eauto. econstructor. eauto.
-    + auto.
-  - destruct Σ as (Σ, univs).
-    unfold erases_global in Heg.
-    assert (Σ ;;; [] |- tConst c u ▷ res) by eauto.
-    eapply inversion_Const in Hty as (? & ? & ? & ? & ?).
-    inv He.
-    + assert (H' := H).
-      eapply lookup_env_erases in H; eauto.
-      destruct H as (decl' & ? & ?).
-      unfold erases_constant_body in H2. rewrite H0 in *.
-      destruct ?; try tauto. cbn in *.
-      eapply declared_constant_inj in d; eauto; subst.
-      edestruct IHeval.
-      * cbn in *.
-        eapply PCUICWeakeningEnv.declared_constant_inv in H'; eauto.
-        unfold on_constant_decl in H'. rewrite H0 in H'. red in H'.
-        eapply typing_subst_instance in H'; eauto.
-        eapply PCUICWeakeningEnv.weaken_env_prop_typing.
-      * eapply PCUICWeakeningEnv.declared_constant_inv in H'; eauto.
-        unfold on_constant_decl in H'. rewrite H0 in H'. cbn in *.
-        2:eapply PCUICWeakeningEnv.weaken_env_prop_typing.
-        eapply erases_subst_instance_constr in H'; eauto.
-      * destruct H3. exists x0. split; eauto. econstructor; eauto.
-    + exists tBox. split. econstructor.
-      eapply Is_type_eval. 3: eassumption. eauto. eauto. econstructor. eauto.
-    + auto.
-  - pose (Hty' := Hty).
-    eapply inversion_Proj in Hty' as (? & ? & ? & [] & ? & ? & ? & ? & ?).
-    inv He.
-    + rename H7 into H6. eapply IHeval1 in H6 as (vc' & Hvc' & Hty_vc'); eauto.
-      eapply erases_mkApps_inv in Hvc'; eauto.
-      2: eapply subject_reduction_eval; eauto.
-      destruct Hvc' as [ (? & ? & ? & ? & [] & ? & ? & ?) | (? & ? & ? & ? & ?)]; subst.
-      * exists tBox. split.
+    + auto. *)
+  - (* Stuck fixpoints are not possible *)
+    unfold isStuckFix in H1.
+    assert (Hty' := Hty).
+    eapply type_mkApps_inv in Hty' as (? & ? & [] & ?); eauto.
+    assert (HT := t).
+    eapply subject_reduction_eval in t; eauto.
+    eapply inversion_Fix in t as (? & ? & ? & ? & ? & ?).
+    unfold unfold_fix in H1. rewrite e in H1.
+    destruct ?; try discriminate. destruct p as [narg fn].
+    destruct ?; try discriminate. inv E.
+    2:auto.
+    eapply nth_error_all in a0; eauto.
+    simpl in a0.
+    destruct a0.
+    rewrite fix_context_length in t.
+    unfold is_constructor in H1. destruct ?; try discriminate.
+    * (* typing_spine x args x0 -> typing spine (dtype x1) args' x0' *)
+      (* Inversions: typing_spine Σ [] (dtype x1) args' x0' -> nth_error args' n = Some t1 ->
+       [ ] |- t1 : tInd _ _.
+       []   |- t1 : tInd -> isConstructapp t1.
+       *)
+      admit.
+    * simpl in H1.
+      (* Under-applied fixpoint is a valid value *)
+      specialize (IHeval _ HT).
+      eapply erases_mkApps_inv in He as [(? & ? & ? & ? & [] & ? & ? & ?) | (? & ? & ? & ? & ?)]; eauto.
+      ** subst.
+         exists tBox. split; auto.
+         admit.
+         admit.
+      ** subst.
+         admit.
 
-        eapply Is_type_app in X as []; eauto. 2:{ rewrite mkApps_nested. eapply subject_reduction_eval; eauto. }
-        rewrite mkApps_nested in X.
-
-        eapply tConstruct_no_Type in X. eapply H5 in X as [? []]; eauto.
-        2: now destruct d. 2: now exists []; destruct Σ.
-
-        econstructor.
-        eapply Is_type_eval. eauto. eauto.
-        eapply nth_error_all.
-        erewrite nth_error_skipn. reflexivity. eassumption.
-        eapply All_impl. assert (pars = ind_npars x0). destruct d as (? & ? & ?). now rewrite H9. subst.
-        eassumption.
-        eapply isErasable_Proof. eauto.
-
-        eapply eval_proj_box.
-        pose proof (Ee.eval_to_value _ _ _ Hty_vc').
-        eapply value_app_inv in H3. subst. eassumption.
-      * rename H5 into Hinf.
-        rename H6 into H5.
-        eapply Forall2_nth_error_Some in H5 as (? & ? & ?); eauto.
-        assert (Σ ;;; [] |- mkApps (tConstruct i k u) args : mkApps (tInd i x) x2).
-        eapply subject_reduction_eval; eauto.
-        eapply type_mkApps_inv in X as (? & ? & [] & ?); eauto.
-        eapply typing_spine_inv in t2 as []; eauto.
-        eapply IHeval2 in H5 as (? & ? & ?); eauto.
-        inv H4.
-        -- exists x9. split; eauto. econstructor. eauto.
-           rewrite <- nth_default_eq. unfold nth_default. now rewrite H3.
-        -- exists tBox. split.
-
-
-           eapply Is_type_app in X as []; eauto. 2:{ eapply subject_reduction_eval. 3: eauto. eauto. eauto. }
-
-           eapply tConstruct_no_Type in X. eapply Hinf in X as [? []]; eauto.
-           2: now destruct d. 2: now exists []; destruct Σ.
-
-           econstructor.
-           eapply Is_type_eval. eauto. eauto.
-           eapply nth_error_all.
-           erewrite nth_error_skipn. reflexivity. eassumption.
-           eapply All_impl. assert (pars = ind_npars x0). destruct d as (? & ? & ?). now rewrite H9. subst.
-           eassumption.
-           eapply isErasable_Proof. eauto.
-
-           eapply eval_proj_box.
-           pose proof (Ee.eval_to_value _ _ _ Hty_vc').
-           eapply value_app_inv in H4. subst. eassumption.
-    + exists tBox. split. econstructor.
-      eapply Is_type_eval. 3: eassumption. eauto. eauto. econstructor. eauto.
-    + auto.
-  - inv He.
-    + eexists. split; eauto. econstructor. constructor.
+  - (* Case Cofix *) admit.
+  - (* Proj cofix *) admit.
+  - (* App congruence *) admit.
+  - admit.
+(*  - inv He.
+    + eexists. split; eauto. econstructor. eauto. constructor.
     + eexists. split; eauto. now econstructor.
   - inv He. eexists. split; eauto. now econstructor.
   - inv He. eexists. split; eauto. now econstructor.
@@ -961,5 +1010,5 @@ Proof.
         -- inv H3. eauto.
         -- inv H3. inv t0. eapply IHAll2 in H5 as (? & ? & ?).
            eapply r in H2 as (? & ? & ?); eauto.
-           eauto.
+           eauto. *)
 Admitted.
